cleaned up simulation definitions and type classes, now complete substitutes for ghost lemmas in Net

core/Simul.v
@@ -20,164 +20,22 @@ Require Import ssreflect.
 
 Set Implicit Arguments.
 
-Class BaseParamsEqMap (P0 : BaseParams) (P1 : BaseParams) := 
+Class BaseParamsTotMap (P0 : BaseParams) (P1 : BaseParams) := 
   {
-    eq_map_data : @data P0 -> @data P1 ;
-    eq_map_input : @input P0 -> @input P1 ;
-    eq_map_output : @output P0 -> @output P1
+    tot_map_data : @data P0 -> @data P1 ;
+    tot_map_input : @input P0 -> @input P1 ;
+    tot_map_output : @output P0 -> @output P1
   }.
 
-Class MultiParamsEqMap
+Class MultiParamsTotMap
  (B0 : BaseParams) (B1 : BaseParams) 
- (B : BaseParamsEqMap B0 B1)
+ (B : BaseParamsTotMap B0 B1)
  (P0 : MultiParams B0) (P1 : MultiParams B1)  :=
 {
-   eq_map_msg : @msg B0 P0 -> @msg B1 P1 ;
-   eq_map_name : @name B0 P0 -> @name B1 P1 ;
-   eq_map_name_inv : @name B1 P1 -> @name B0 P0 ;
-   eq_map_name_inv_inverse : forall n, eq_map_name_inv (eq_map_name n) = n ;
-   eq_map_name_inverse_inv : forall n, eq_map_name (eq_map_name_inv n) = n
+   tot_map_msg : @msg B0 P0 -> @msg B1 P1 ;
+   tot_map_name : @name B0 P0 -> @name B1 P1 ;
+   tot_map_name_inv : @name B1 P1 -> @name B0 P0
 }.
-
-Section SimulOneToOne.
-
-Context {base_fst : BaseParams}.
-Context {base_snd : BaseParams}.
-Context {multi_fst : MultiParams base_fst}.
-Context {multi_snd : MultiParams base_snd}.
-Context {base_map : BaseParamsEqMap base_fst base_snd}.
-Context {multi_map : MultiParamsEqMap base_map multi_fst multi_snd}.
-
-Definition eq_mapped_init_handlers n := 
-  eq_map_data (init_handlers n).
-
-Hypothesis eq_mapped_init_handlers_eq : forall n,
-  eq_mapped_init_handlers n = init_handlers (eq_map_name n).
-
-Definition eq_map_name_msgs :=
-  map (fun nm => (eq_map_name (fst nm), eq_map_msg (snd nm))).
-
-Definition eq_mapped_net_handlers me src m st :=
-  let '(out, st', ps) := net_handlers me src m st in
-  (map eq_map_output out, eq_map_data st', eq_map_name_msgs ps).
-
-Hypothesis eq_net_handlers_eq : forall me src m st,
-  eq_mapped_net_handlers me src m st = 
-  net_handlers (eq_map_name me) (eq_map_name src) (eq_map_msg m) (eq_map_data st).
-
-Definition eq_mapped_input_handlers me inp st :=
-  let '(out, st', ps) := input_handlers me inp st in
-  (map eq_map_output out, eq_map_data st', eq_map_name_msgs ps).
-
-Hypothesis eq_input_handlers_eq : forall me inp st,
-  eq_mapped_input_handlers me inp st = input_handlers (eq_map_name me) (eq_map_input inp) (eq_map_data st).
-
-Definition eq_map_trace_occ (e : @name _ multi_fst * (@input base_fst + list (@output base_fst))) :=
-match e with
-| (n, inl io) => (eq_map_name n, inl (eq_map_input io))
-| (n, inr lo) => (eq_map_name n, inr (map eq_map_output lo))
-end.
-
-Definition eq_map_packet (p : @packet base_fst multi_fst)  :=
-match p with
-| mkPacket src dst m =>
-  mkPacket (eq_map_name src) (eq_map_name dst) (eq_map_msg m)
-end.
-
-Definition eq_map_net (net : @network _ multi_fst) : @network _ multi_snd :=
-mkNetwork (map eq_map_packet net.(nwPackets)) (fun n => eq_map_data (net.(nwState) (eq_map_name_inv n))).
-
-Lemma eq_map_update_eq :
-  forall net d h,
-    (fun n : name => eq_map_data (update (nwState net) h d (eq_map_name_inv n))) =
-    update (fun n : name => eq_map_data (nwState net (eq_map_name_inv n))) (eq_map_name h) (eq_map_data d).
-Proof.
-move => net d h.
-apply functional_extensionality => n.
-rewrite /update /=.
-case (name_eq_dec _ _) => H_dec; case (name_eq_dec _ _) => H_dec' //.
-  rewrite -H_dec in H_dec'.
-  by rewrite eq_map_name_inverse_inv in H_dec'.
-rewrite H_dec' in H_dec.
-by rewrite eq_map_name_inv_inverse in H_dec.
-Qed.
-
-Corollary eq_map_update_packet_eq :
-forall net p d,
-  (fun n : name => eq_map_data (update (nwState net) (pDst p) d (eq_map_name_inv n))) =
-  (update (fun n : name => eq_map_data (nwState net (eq_map_name_inv n))) (pDst (eq_map_packet p)) (eq_map_data d)).
-Proof.
-move => net. 
-case => src dst m d.
-exact: eq_map_update_eq.
-Qed.
-
-Lemma eq_map_packet_app_eq :
-  forall l p ms ms',
-    map eq_map_packet (map (fun m : name * msg => {| pSrc := pDst p; pDst := fst m; pBody := snd m |}) l ++ ms ++ ms') = 
-    map (fun m : name * msg => {| pSrc := pDst (eq_map_packet p); pDst := fst m; pBody := snd m |}) (eq_map_name_msgs l) ++ map eq_map_packet ms ++ map eq_map_packet ms'.
-Proof.
-move => l; case => src dst m ms ms'.
-rewrite 2!map_app.
-elim: l => //=.
-case => /= n m' l IH.
-by rewrite IH.
-Qed.
-
-Lemma eq_map_packet_eq :
-  forall l l' h,
-    map eq_map_packet (map (fun m : name * msg => {| pSrc := h; pDst := fst m; pBody := snd m |}) l ++ l') =
-    map (fun m : name * msg => {| pSrc := eq_map_name h; pDst := fst m; pBody := snd m |}) (eq_map_name_msgs l) ++ map eq_map_packet l'.
-Proof.
-elim => //=.
-case => n m l IH l' h.
-by rewrite IH.
-Qed.
-
-Lemma init_handlers_fun_eq : 
-    init_handlers = fun n : name => eq_map_data (init_handlers (eq_map_name_inv n)).
-Proof.
-apply functional_extensionality => n.
-have H_eq := eq_mapped_init_handlers_eq.
-rewrite /eq_mapped_init_handlers in H_eq.
-rewrite H_eq {H_eq}.
-by rewrite eq_map_name_inverse_inv.
-Qed.
-
-Theorem step_m_eq_mapped_simulation_1 :
-  forall net net' tr,
-    @step_m _ multi_fst net net' tr ->
-    @step_m _ multi_snd (eq_map_net net) (eq_map_net net') (map eq_map_trace_occ tr).
-Proof.
-move => net net' tr.
-case => {net net' tr}.
-- move => net net' p ms ms' out d l H_eq H_hnd H_eq'.
-  rewrite /eq_map_trace_occ /=.
-  have ->: eq_map_name (pDst p) = pDst (eq_map_packet p) by case: p H_eq H_hnd H_eq' => src dst m H_eq H_hnd H_eq'.
-  apply (@SM_deliver _ _ _ _ _ (map eq_map_packet ms) (map eq_map_packet ms') (map eq_map_output out) (eq_map_data d) (eq_map_name_msgs l)).
-  * by rewrite /eq_map_net /= H_eq /= map_app.
-  * rewrite /=.
-    case: p H_eq H_hnd H_eq' => /= src dst m H_eq H_hnd H_eq'.
-    have H_q := eq_net_handlers_eq dst src m (nwState net dst).
-    rewrite /eq_mapped_net_handlers in H_q.
-    rewrite H_hnd in H_q.
-    rewrite H_q.
-    by rewrite eq_map_name_inv_inverse.
-  * rewrite /= H_eq' /= /eq_map_net /=.
-    rewrite -eq_map_update_packet_eq.
-    by rewrite eq_map_packet_app_eq.
-- move => h net net' out inp d l H_hnd H_eq.
-  apply (@SM_input _ _ _ _ _ _ _ (eq_map_data d) (eq_map_name_msgs l)).
-    rewrite /=.
-    have H_q := eq_input_handlers_eq h inp (nwState net h).
-    rewrite /eq_mapped_input_handlers /= in H_q.
-    rewrite H_hnd in H_q.
-    rewrite H_q.
-    by rewrite eq_map_name_inv_inverse.
-  rewrite /= H_eq /= /eq_map_net /=.
-  rewrite -eq_map_update_eq.
-  by rewrite eq_map_packet_eq.
-Qed.
 
 Lemma map_eq_inv :
   forall (A B : Type) (f : A -> B) (l : list A) xs ys,
@@ -213,58 +71,6 @@ elim => /=.
     by rewrite H_eq_l H_eq_l1 H_eq_l2.
 Qed.
 
-Lemma eq_map_trace_occ_inv : 
-  forall tr n ol,
-    map eq_map_trace_occ tr = [(n, inr ol)] -> 
-    exists n', exists lo, tr = [(n', inr lo)] /\ eq_map_name n' = n /\ map eq_map_output lo = ol.
-Proof.
-case => //=.
-case.
-move => n ol tr n' lo H_eq.
-case: tr H_eq => //=.
-case: ol => //=.
-move => out H_eq.
-exists n; exists out.
-split => //.
-by inversion H_eq.
-Qed.
-
-Lemma eq_map_name_injective : 
-forall n n', eq_map_name n = eq_map_name n' -> n = n'.
-Proof.
-move => n n'.
-case (name_eq_dec n n') => H_dec //.
-move => H_eq.
-rewrite -(eq_map_name_inv_inverse n) in H_dec.
-rewrite H_eq in H_dec.
-by rewrite eq_map_name_inv_inverse in H_dec.
-Qed.
-
-Lemma eq_map_trace_occ_in_inv : 
-  forall tr h inp out,
-    map eq_map_trace_occ tr = [(h, inl inp); (h, inr out)] -> 
-    exists h', exists inp', exists out', tr = [(h', inl inp'); (h', inr out')] /\ 
-      eq_map_name h' = h /\ map eq_map_output out' = out /\ eq_map_input inp' = inp.
-Proof.
-case => //=.
-case.
-move => h.
-case => //.
-move => inp.
-case => //.
-case.
-move => h'.
-case => //.
-move => out.
-case => //=.
-move => h0.
-move => inp' out' H_eq.
-inversion H_eq; subst.
-apply eq_map_name_injective in H2.
-rewrite H2.
-by exists h; exists inp; exists out.
-Qed.
-
 Lemma map_eq_inv_eq :
   forall (A B : Type) (f : A -> B),
     (forall a a', f a = f a' -> a = a') ->
@@ -281,22 +87,228 @@ apply H_inj in H0.
 by rewrite H0 H_eq'.
 Qed.
 
-Hypothesis eq_map_output_injective : 
-  forall o o', eq_map_output o = eq_map_output o' -> o = o'.
+Lemma map_fst_snd_id : 
+  forall A B l, map (fun t : A * B => (fst t, snd t)) l = l.
+Proof.
+move => A B.
+elim => //.
+move => a l IH.
+rewrite /= IH.
+by case: a.
+Qed.
 
-Theorem step_m_eq_mapped_simulation_2 :
+Section SimulTot.
+
+Context {base_fst : BaseParams}.
+Context {base_snd : BaseParams}.
+Context {multi_fst : MultiParams base_fst}.
+Context {multi_snd : MultiParams base_snd}.
+Context {base_map : BaseParamsTotMap base_fst base_snd}.
+Context {multi_map : MultiParamsTotMap base_map multi_fst multi_snd}.
+
+Hypothesis tot_map_name_inv_inverse : forall n, tot_map_name_inv (tot_map_name n) = n.
+
+Hypothesis tot_map_name_inverse_inv : forall n, tot_map_name (tot_map_name_inv n) = n.
+
+Definition tot_mapped_init_handlers n := 
+  tot_map_data (init_handlers n).
+
+Hypothesis tot_mapped_init_handlers_eq : forall n,
+  tot_mapped_init_handlers n = init_handlers (tot_map_name n).
+
+Definition tot_map_name_msgs :=
+  map (fun nm => (tot_map_name (fst nm), tot_map_msg (snd nm))).
+
+Definition tot_mapped_net_handlers me src m st :=
+  let '(out, st', ps) := net_handlers me src m st in
+  (map tot_map_output out, tot_map_data st', tot_map_name_msgs ps).
+
+Hypothesis eq_net_handlers_eq : forall me src m st,
+  tot_mapped_net_handlers me src m st = 
+  net_handlers (tot_map_name me) (tot_map_name src) (tot_map_msg m) (tot_map_data st).
+
+Definition tot_mapped_input_handlers me inp st :=
+  let '(out, st', ps) := input_handlers me inp st in
+  (map tot_map_output out, tot_map_data st', tot_map_name_msgs ps).
+
+Hypothesis eq_input_handlers_eq : forall me inp st,
+  tot_mapped_input_handlers me inp st = input_handlers (tot_map_name me) (tot_map_input inp) (tot_map_data st).
+
+Definition tot_map_trace_occ (e : @name _ multi_fst * (@input base_fst + list (@output base_fst))) :=
+match e with
+| (n, inl io) => (tot_map_name n, inl (tot_map_input io))
+| (n, inr lo) => (tot_map_name n, inr (map tot_map_output lo))
+end.
+
+Definition tot_map_packet (p : @packet base_fst multi_fst)  :=
+match p with
+| mkPacket src dst m =>
+  mkPacket (tot_map_name src) (tot_map_name dst) (tot_map_msg m)
+end.
+
+Definition tot_map_net (net : @network _ multi_fst) : @network _ multi_snd :=
+mkNetwork (map tot_map_packet net.(nwPackets)) (fun n => tot_map_data (net.(nwState) (tot_map_name_inv n))).
+
+Lemma tot_map_update_eq :
+  forall net d h,
+    (fun n : name => tot_map_data (update (nwState net) h d (tot_map_name_inv n))) =
+    update (fun n : name => tot_map_data (nwState net (tot_map_name_inv n))) (tot_map_name h) (tot_map_data d).
+Proof.
+move => net d h.
+apply functional_extensionality => n.
+rewrite /update /=.
+case (name_eq_dec _ _) => H_dec; case (name_eq_dec _ _) => H_dec' //.
+  rewrite -H_dec in H_dec'.
+  by rewrite tot_map_name_inverse_inv in H_dec'.
+rewrite H_dec' in H_dec.
+by rewrite tot_map_name_inv_inverse in H_dec.
+Qed.
+
+Corollary tot_map_update_packet_eq :
+forall net p d,
+  (fun n : name => tot_map_data (update (nwState net) (pDst p) d (tot_map_name_inv n))) =
+  (update (fun n : name => tot_map_data (nwState net (tot_map_name_inv n))) (pDst (tot_map_packet p)) (tot_map_data d)).
+Proof.
+move => net. 
+case => src dst m d.
+exact: tot_map_update_eq.
+Qed.
+
+Lemma tot_map_packet_app_eq :
+  forall l p ms ms',
+    map tot_map_packet (map (fun m : name * msg => {| pSrc := pDst p; pDst := fst m; pBody := snd m |}) l ++ ms ++ ms') = 
+    map (fun m : name * msg => {| pSrc := pDst (tot_map_packet p); pDst := fst m; pBody := snd m |}) (tot_map_name_msgs l) ++ map tot_map_packet ms ++ map tot_map_packet ms'.
+Proof.
+move => l; case => src dst m ms ms'.
+rewrite 2!map_app.
+elim: l => //=.
+case => /= n m' l IH.
+by rewrite IH.
+Qed.
+
+Lemma tot_map_packet_eq :
+  forall l l' h,
+    map tot_map_packet (map (fun m : name * msg => {| pSrc := h; pDst := fst m; pBody := snd m |}) l ++ l') =
+    map (fun m : name * msg => {| pSrc := tot_map_name h; pDst := fst m; pBody := snd m |}) (tot_map_name_msgs l) ++ map tot_map_packet l'.
+Proof.
+elim => //=.
+case => n m l IH l' h.
+by rewrite IH.
+Qed.
+
+Lemma init_handlers_fun_eq : 
+    init_handlers = fun n : name => tot_map_data (init_handlers (tot_map_name_inv n)).
+Proof.
+apply functional_extensionality => n.
+have H_eq := tot_mapped_init_handlers_eq.
+rewrite /tot_mapped_init_handlers in H_eq.
+rewrite H_eq {H_eq}.
+by rewrite tot_map_name_inverse_inv.
+Qed.
+
+Theorem step_m_tot_mapped_simulation_1 :
+  forall net net' tr,
+    @step_m _ multi_fst net net' tr ->
+    @step_m _ multi_snd (tot_map_net net) (tot_map_net net') (map tot_map_trace_occ tr).
+Proof.
+move => net net' tr.
+case => {net net' tr}.
+- move => net net' p ms ms' out d l H_eq H_hnd H_eq'.
+  rewrite /tot_map_trace_occ /=.
+  have ->: tot_map_name (pDst p) = pDst (tot_map_packet p) by case: p H_eq H_hnd H_eq' => src dst m H_eq H_hnd H_eq'.
+  apply (@SM_deliver _ _ _ _ _ (map tot_map_packet ms) (map tot_map_packet ms') (map tot_map_output out) (tot_map_data d) (tot_map_name_msgs l)).
+  * by rewrite /tot_map_net /= H_eq /= map_app.
+  * rewrite /=.
+    case: p H_eq H_hnd H_eq' => /= src dst m H_eq H_hnd H_eq'.
+    have H_q := eq_net_handlers_eq dst src m (nwState net dst).
+    rewrite /tot_mapped_net_handlers in H_q.
+    rewrite H_hnd in H_q.
+    rewrite H_q.
+    by rewrite tot_map_name_inv_inverse.
+  * rewrite /= H_eq' /= /tot_map_net /=.
+    rewrite -tot_map_update_packet_eq.
+    by rewrite tot_map_packet_app_eq.
+- move => h net net' out inp d l H_hnd H_eq.
+  apply (@SM_input _ _ _ _ _ _ _ (tot_map_data d) (tot_map_name_msgs l)).
+    rewrite /=.
+    have H_q := eq_input_handlers_eq h inp (nwState net h).
+    rewrite /tot_mapped_input_handlers /= in H_q.
+    rewrite H_hnd in H_q.
+    rewrite H_q.
+    by rewrite tot_map_name_inv_inverse.
+  rewrite /= H_eq /= /tot_map_net /=.
+  rewrite -tot_map_update_eq.
+  by rewrite tot_map_packet_eq.
+Qed.
+
+Lemma tot_map_trace_occ_inv : 
+  forall tr n ol,
+    map tot_map_trace_occ tr = [(n, inr ol)] -> 
+    exists n', exists lo, tr = [(n', inr lo)] /\ tot_map_name n' = n /\ map tot_map_output lo = ol.
+Proof.
+case => //=.
+case.
+move => n ol tr n' lo H_eq.
+case: tr H_eq => //=.
+case: ol => //=.
+move => out H_eq.
+exists n; exists out.
+split => //.
+by inversion H_eq.
+Qed.
+
+Lemma tot_map_name_injective : 
+forall n n', tot_map_name n = tot_map_name n' -> n = n'.
+Proof.
+move => n n'.
+case (name_eq_dec n n') => H_dec //.
+move => H_eq.
+rewrite -(tot_map_name_inv_inverse n) in H_dec.
+rewrite H_eq in H_dec.
+by rewrite tot_map_name_inv_inverse in H_dec.
+Qed.
+
+Lemma tot_map_trace_occ_in_inv : 
+  forall tr h inp out,
+    map tot_map_trace_occ tr = [(h, inl inp); (h, inr out)] -> 
+    exists h', exists inp', exists out', tr = [(h', inl inp'); (h', inr out')] /\ 
+      tot_map_name h' = h /\ map tot_map_output out' = out /\ tot_map_input inp' = inp.
+Proof.
+case => //=.
+case.
+move => h.
+case => //.
+move => inp.
+case => //.
+case.
+move => h'.
+case => //.
+move => out.
+case => //=.
+move => h0.
+move => inp' out' H_eq.
+inversion H_eq; subst.
+apply tot_map_name_injective in H2.
+rewrite H2.
+by exists h; exists inp; exists out.
+Qed.
+
+Hypothesis tot_map_output_injective : 
+  forall o o', tot_map_output o = tot_map_output o' -> o = o'.
+
+Theorem step_m_tot_mapped_simulation_2 :
   forall net net' out mnet mout,
       @step_m _ multi_snd net net' out ->
-      eq_map_net mnet = net ->
-      map eq_map_trace_occ mout = out ->
+      tot_map_net mnet = net ->
+      map tot_map_trace_occ mout = out ->
       exists mnet',
         @step_m _ multi_fst mnet mnet' mout /\
-        eq_map_net mnet' = net'.
+        tot_map_net mnet' = net'.
 Proof.
 move => net net' out mnet mout H_step H_eq H_eq'.
 invcs H_step.
 - case: p H4 H H0 => /= src dst m H4 H H0.
-  rewrite /eq_map_net /=.
+  rewrite /tot_map_net /=.
   case: mnet H H0 => /= pks sts H_eq H_hnd.
   have [pks1 [pks2 [H_eq_pks [H_eq_pks1 H_eq_pks2]]]] := map_eq_inv _ _ _ _ H_eq.
   case: pks2 H_eq_pks H_eq_pks2 => //= p pks2 H_eq_pks H_eq_pks2.
@@ -307,35 +319,35 @@ invcs H_step.
   rewrite -H_eq_pks1.
   exists {| nwPackets := send_packets (pDst p) l' ++ pks1 ++ pks2 ; nwState := update sts (pDst p) d' |}.
   split.
-  * have [n' [lo [H_eq_mout [H_eq_n H_eq_lo]]]] := eq_map_trace_occ_inv _ (eq_sym H4).
+  * have [n' [lo [H_eq_mout [H_eq_n H_eq_lo]]]] := tot_map_trace_occ_inv _ (eq_sym H4).
     rewrite H_eq_mout.
     have H_eq_dst: n' = pDst p.
-      rewrite -(eq_map_name_inv_inverse n').
+      rewrite -(tot_map_name_inv_inverse n').
       rewrite H_eq_n.
       case: p H_eq_pks H_eq_pks2 H0 H_hnd' => src' dst' m' H_eq_pks H_eq_pks2 H0 H_hnd'.
       rewrite /=.
       rewrite /= in H0.
       inversion H0.
-      by rewrite eq_map_name_inv_inverse.
+      by rewrite tot_map_name_inv_inverse.
     rewrite H_eq_dst.
     apply (@SM_deliver _ _ _ _ _ pks1 pks2 _ d' l') => //=.
     suff H_suff: lo = out' by rewrite H_suff.
     have H_eq_hnd := eq_net_handlers_eq (pDst p) (pSrc p) (pBody p) (sts (pDst p)).
-    rewrite /eq_mapped_net_handlers /= in H_eq_hnd.
+    rewrite /tot_mapped_net_handlers /= in H_eq_hnd.
     repeat break_let.
     inversion H_hnd'.
     rewrite H2 H3 H5 in H_eq_hnd.
     rewrite -{1}H_eq_dst H_eq_n in H_eq_hnd.
     rewrite -H_eq_dst in H_eq_hnd.
-    rewrite -(eq_map_name_inv_inverse n') H_eq_n in H_eq_hnd.
+    rewrite -(tot_map_name_inv_inverse n') H_eq_n in H_eq_hnd.
     move {Heqp1 Heqp0 H_hnd'}.
-    have H_eq_src: eq_map_name (pSrc p) = src.
+    have H_eq_src: tot_map_name (pSrc p) = src.
       case: p H_eq_pks H_eq_pks2 H0 H_eq_dst H_eq_hnd => src' dst' m' H_eq_pks H_eq_pks2 H0 H_eq_dst H_eq_hnd.
       rewrite /=.
       rewrite /= in H0.
       by inversion H0.
     rewrite H_eq_src /= {H_eq_src} in H_eq_hnd.
-    have H_eq_body: eq_map_msg (pBody p) = m.
+    have H_eq_body: tot_map_msg (pBody p) = m.
       case: p H_eq_pks H_eq_pks2 H0 H_eq_dst H_eq_hnd => src' dst' m' H_eq_pks H_eq_pks2 H0 H_eq_dst H_eq_hnd.
       rewrite /=.
       rewrite /= in H0.
@@ -346,33 +358,33 @@ invcs H_step.
     symmetry.
     move: H6.
     apply map_eq_inv_eq.
-    exact: eq_map_output_injective.
+    exact: tot_map_output_injective.
   * rewrite /=.
     rewrite /update /=.
-    have H_eq_dst: eq_map_name (pDst p) = dst.
+    have H_eq_dst: tot_map_name (pDst p) = dst.
       case: p H_eq_pks H_eq_pks2 H0 H_hnd' => src' dst' m' H_eq_pks H_eq_pks2 H0 H_hnd'.
       by inversion H0.
-    have H_eq_src: eq_map_name (pSrc p) = src.
+    have H_eq_src: tot_map_name (pSrc p) = src.
       case: p H_eq_pks H_eq_pks2 H0 H_hnd' H_eq_dst => src' dst' m' H_eq_pks H_eq_pks2 H0 H_hnd' H_eq_dst.
       by inversion H0.
-    have H_eq_body: eq_map_msg (pBody p) = m.
+    have H_eq_body: tot_map_msg (pBody p) = m.
       case: p H_eq_pks H_eq_pks2 H0 H_eq_dst H_eq_src H_hnd' => src' dst' m' H_eq_pks H_eq_pks2 H0 H_eq_dst H_eq_src H_hnd'.
       by inversion H0.
     rewrite 2!map_app.
     have H_eq_hnd := eq_net_handlers_eq (pDst p) (pSrc p) (pBody p) (sts (pDst p)).
-    rewrite /eq_mapped_net_handlers /= in H_eq_hnd.
+    rewrite /tot_mapped_net_handlers /= in H_eq_hnd.
     repeat break_let.
     inversion H_hnd'.
     rewrite H_eq_dst H_eq_src H_eq_body in H_eq_hnd.
-    rewrite -{2}H_eq_dst eq_map_name_inv_inverse in H_hnd.
+    rewrite -{2}H_eq_dst tot_map_name_inv_inverse in H_hnd.
     rewrite H_hnd in H_eq_hnd.
     inversion H_eq_hnd.
     rewrite H2 in H6.
     rewrite H3 in H7.
     rewrite H5 in H8.
     rewrite H3 H5.
-    set nwP1 := map eq_map_packet _.
-    set nwP2 := map (fun _ => _) (eq_map_name_msgs _).
+    set nwP1 := map tot_map_packet _.
+    set nwP2 := map (fun _ => _) (tot_map_name_msgs _).
     set nwS1 := fun _ => _.
     set nwS2 := fun _ => _.
     have H_eq_nw: nwP1 = nwP2.
@@ -388,20 +400,20 @@ invcs H_step.
       rewrite -H_eq_dst.
       case (name_eq_dec _ _) => H_dec.
         rewrite -H_dec.
-        rewrite eq_map_name_inverse_inv.
+        rewrite tot_map_name_inverse_inv.
         by case (name_eq_dec _ _).
       case (name_eq_dec _ _) => H_dec' //.
       rewrite H_dec' in H_dec.
-      by rewrite eq_map_name_inv_inverse in H_dec.
+      by rewrite tot_map_name_inv_inverse in H_dec.
     by rewrite H_eq_sw.
-- rewrite /eq_map_net /=.
+- rewrite /tot_map_net /=.
   case: mnet H => /= pks sts H_hnd.
-  have [h' [inp' [out' [H_eq_mout [H_eq_n [H_eq_out H_eq_inp]]]]]] := eq_map_trace_occ_in_inv _ (eq_sym H3).
+  have [h' [inp' [out' [H_eq_mout [H_eq_n [H_eq_out H_eq_inp]]]]]] := tot_map_trace_occ_in_inv _ (eq_sym H3).
   have H_q := eq_input_handlers_eq h' inp' (sts h').
-  rewrite /eq_mapped_input_handlers in H_q.
+  rewrite /tot_mapped_input_handlers in H_q.
   repeat break_let.
   rewrite H_eq_n H_eq_inp in H_q.
-  rewrite -{2}H_eq_n eq_map_name_inv_inverse in H_hnd.
+  rewrite -{2}H_eq_n tot_map_name_inv_inverse in H_hnd.
   rewrite H_hnd in H_q.
   inversion H_q.
   rewrite -H_eq_out in H0.
@@ -414,9 +426,9 @@ invcs H_step.
     suff H_suff: l1 = out' by rewrite H_suff.
     move: H0.
     apply map_eq_inv_eq.
-    exact: eq_map_output_injective.
+    exact: tot_map_output_injective.
   * rewrite /= map_app.
-    set nwP1 := map eq_map_packet _.
+    set nwP1 := map tot_map_packet _.
     set nwP2 := map (fun _ => _) l.
     set nwS1 := fun _ => _.
     set nwS2 := update _ _ _.
@@ -433,13 +445,13 @@ invcs H_step.
       rewrite -H_eq_n -H1.
       case (name_eq_dec _ _) => H_dec.
         case (name_eq_dec _ _) => H_dec' //.
-        by rewrite -H_dec eq_map_name_inverse_inv in H_dec'.
+        by rewrite -H_dec tot_map_name_inverse_inv in H_dec'.
       case (name_eq_dec _ _) => H_dec' //.
-      by rewrite H_dec' eq_map_name_inv_inverse in H_dec.
+      by rewrite H_dec' tot_map_name_inv_inverse in H_dec.
     by rewrite H_eq_nwp H_eq_nws.
 Qed.
 
-Theorem step_m_eq_mapped_invariant_lift :
+Theorem step_m_tot_mapped_invariant_lift :
   forall P : _ -> Prop,
     (forall net net' out,
        @step_m _ multi_snd net net' out ->
@@ -447,44 +459,44 @@ Theorem step_m_eq_mapped_invariant_lift :
        P net') ->
     (forall net net' out,
        @step_m _ multi_fst net net' out ->
-       P (eq_map_net net) ->
-       P (eq_map_net net')).
-Proof. by move => P; eauto using step_m_eq_mapped_simulation_1. Qed.
+       P (tot_map_net net) ->
+       P (tot_map_net net')).
+Proof. by move => P; eauto using step_m_tot_mapped_simulation_1. Qed.
 
-Corollary step_m_mapped_simulation_star_1 :
+Corollary step_m_tot_mapped_simulation_star_1 :
   forall net tr,
     @step_m_star _ multi_fst step_m_init net tr ->
-    @step_m_star _ multi_snd step_m_init (eq_map_net net) (map eq_map_trace_occ tr).
+    @step_m_star _ multi_snd step_m_init (tot_map_net net) (map tot_map_trace_occ tr).
 Proof.
 move => net tr H_step.
 remember step_m_init as y in *.
 move: Heqy.
 induction H_step using refl_trans_1n_trace_n1_ind => H_init /=.
   rewrite H_init.
-  rewrite /step_m_init /= /eq_map_net /=.
+  rewrite /step_m_init /= /tot_map_net /=.
   rewrite init_handlers_fun_eq.
   exact: RT1nTBase.
 concludes.
 rewrite H_init in H_step2 H_step1.
-apply step_m_eq_mapped_simulation_1 in H.
+apply step_m_tot_mapped_simulation_1 in H.
 rewrite map_app.
 have H_trans := refl_trans_1n_trace_trans IHH_step1.
 apply: H_trans.
 rewrite (app_nil_end (map _ _)).
-apply: (@RT1nTStep _ _ _ _ (eq_map_net x'')) => //.
+apply: (@RT1nTStep _ _ _ _ (tot_map_net x'')) => //.
 exact: RT1nTBase.
 Qed.
 
 Context {fail_fst : FailureParams multi_fst}.
 Context {fail_snd : FailureParams multi_snd}.
 
-Hypothesis eq_mapped_reboot_eq : forall d,
-  eq_map_data (reboot d) = reboot (eq_map_data d).
+Hypothesis tot_mapped_reboot_eq : forall d,
+  tot_map_data (reboot d) = reboot (tot_map_data d).
 
 Lemma not_in_failed_not_in :
   forall n failed,
     ~ In n failed ->
-    ~ In (eq_map_name n) (map eq_map_name failed).
+    ~ In (tot_map_name n) (map tot_map_name failed).
 Proof.
 move => n.
 elim => //=.
@@ -492,9 +504,9 @@ move => n' failed IH H_in H_in'.
 case: H_in' => H_in'.
   case: H_in.
   left.
-  rewrite -(eq_map_name_inv_inverse n').
+  rewrite -(tot_map_name_inv_inverse n').
   rewrite H_in'.
-  exact: eq_map_name_inv_inverse.
+  exact: tot_map_name_inv_inverse.
 contradict H_in'.
 apply: IH.
 move => H_in'.
@@ -505,7 +517,7 @@ Qed.
 Lemma in_failed_in :
   forall n failed,
     In n failed ->
-    In (eq_map_name n) (map eq_map_name failed).
+    In (tot_map_name n) (map tot_map_name failed).
 Proof.
 move => n.
 elim => //.
@@ -517,92 +529,92 @@ right.
 exact: IH.
 Qed.
 
-Lemma remove_eq_map_eq :
+Lemma remove_tot_map_eq :
   forall h failed,
-    map eq_map_name (remove name_eq_dec h failed) =
-    remove name_eq_dec (eq_map_name h) (map eq_map_name failed).
+    map tot_map_name (remove name_eq_dec h failed) =
+    remove name_eq_dec (tot_map_name h) (map tot_map_name failed).
 Proof.
 move => h.
 elim => //=.
 move => n failed IH.
 case (name_eq_dec _ _) => H_eq; case (name_eq_dec _ _) => H_eq' //.
 - by rewrite H_eq in H_eq'.
-- rewrite -(eq_map_name_inv_inverse h) in H_eq.
+- rewrite -(tot_map_name_inv_inverse h) in H_eq.
   rewrite H_eq' in H_eq.
-  by rewrite eq_map_name_inv_inverse in H_eq.
+  by rewrite tot_map_name_inv_inverse in H_eq.
 - by rewrite /= IH.
 Qed.
 
-Lemma eq_map_reboot_eq :
+Lemma tot_map_reboot_eq :
 forall h net,
     (fun n : name => 
-      eq_map_data 
-        (match name_eq_dec (eq_map_name_inv n) h with
-         | left _ => reboot (nwState net (eq_map_name_inv n))
-         | right _ => nwState net (eq_map_name_inv n)
+      tot_map_data 
+        (match name_eq_dec (tot_map_name_inv n) h with
+         | left _ => reboot (nwState net (tot_map_name_inv n))
+         | right _ => nwState net (tot_map_name_inv n)
         end)) =
     (fun nm : name =>
-       match name_eq_dec nm (eq_map_name h) with
-       | left _ => reboot (eq_map_data (nwState net (eq_map_name_inv nm)))
-       | right _ => eq_map_data (nwState net (eq_map_name_inv nm))
+       match name_eq_dec nm (tot_map_name h) with
+       | left _ => reboot (tot_map_data (nwState net (tot_map_name_inv nm)))
+       | right _ => tot_map_data (nwState net (tot_map_name_inv nm))
        end).
 Proof.
 move => h net.
 apply: functional_extensionality => n.
 case (name_eq_dec _ _) => H_dec; case (name_eq_dec _ _) => H_dec' //.
 - rewrite -H_dec in H_dec'.
-  by rewrite eq_map_name_inverse_inv in H_dec'.
+  by rewrite tot_map_name_inverse_inv in H_dec'.
 - rewrite H_dec' in H_dec.
-  by rewrite eq_map_name_inv_inverse in H_dec.
+  by rewrite tot_map_name_inv_inverse in H_dec.
 Qed.
 
-Theorem step_f_eq_mapped_simulation_1 :
+Theorem step_f_tot_mapped_simulation_1 :
   forall net net' failed failed' tr,
     @step_f _ _ fail_fst (failed, net) (failed', net') tr ->
-    @step_f _ _ fail_snd (map eq_map_name failed, eq_map_net net) (map eq_map_name failed', eq_map_net net') (map eq_map_trace_occ tr).
+    @step_f _ _ fail_snd (map tot_map_name failed, tot_map_net net) (map tot_map_name failed', tot_map_net net') (map tot_map_trace_occ tr).
 Proof.
 move => net net' failed failed' tr H_step.
 invcs H_step.
-- have ->: eq_map_name (pDst p) = pDst (eq_map_packet p) by case: p H3 H4 H6 => src dst m.
-  apply (@SF_deliver _ _ _ _ _ _ _ (map eq_map_packet xs) (map eq_map_packet ys) _ (eq_map_data d) (eq_map_name_msgs l)).
-  * by rewrite /eq_map_net /= H3 /= map_app.
+- have ->: tot_map_name (pDst p) = pDst (tot_map_packet p) by case: p H3 H4 H6 => src dst m.
+  apply (@SF_deliver _ _ _ _ _ _ _ (map tot_map_packet xs) (map tot_map_packet ys) _ (tot_map_data d) (tot_map_name_msgs l)).
+  * by rewrite /tot_map_net /= H3 /= map_app.
   * case: p H3 H4 H6 => /= src dst m H3 H4 H6.
     exact: not_in_failed_not_in.
   * case: p H3 H4 H6 => /= src dst m H3 H4 H6.        
     have H_q := eq_net_handlers_eq dst src m (nwState net dst).
-    rewrite /eq_mapped_net_handlers in H_q.
+    rewrite /tot_mapped_net_handlers in H_q.
     rewrite H6 in H_q.
     rewrite H_q.
-    by rewrite eq_map_name_inv_inverse.
-  * rewrite /= -eq_map_update_packet_eq /=.
-    rewrite /eq_map_net /=.
-    by rewrite eq_map_packet_app_eq.
-- apply (@SF_input _ _ _ _ _ _ _ _ _ (eq_map_data d) (eq_map_name_msgs l)).
+    by rewrite tot_map_name_inv_inverse.
+  * rewrite /= -tot_map_update_packet_eq /=.
+    rewrite /tot_map_net /=.
+    by rewrite tot_map_packet_app_eq.
+- apply (@SF_input _ _ _ _ _ _ _ _ _ (tot_map_data d) (tot_map_name_msgs l)).
   * exact: not_in_failed_not_in.
   * rewrite /=.
     have H_q := eq_input_handlers_eq h inp (nwState net h).
-    rewrite /eq_mapped_input_handlers /= in H_q.
+    rewrite /tot_mapped_input_handlers /= in H_q.
     rewrite H5 in H_q.
     rewrite H_q.
-    by rewrite eq_map_name_inv_inverse.
-  * rewrite /= /eq_map_net /=.
-    rewrite -eq_map_update_eq.
-    by rewrite eq_map_packet_eq.
-- apply (@SF_drop _ _ _ _ _ _ (eq_map_packet p) (map eq_map_packet xs) (map eq_map_packet ys)).
-  * by rewrite /eq_map_net /= H4 map_app.
-  * by rewrite /eq_map_net /= map_app.
-- apply (@SF_dup _ _ _ _ _ _ (eq_map_packet p) (map eq_map_packet xs) (map eq_map_packet ys)).
-  * by rewrite /eq_map_net /= H4 map_app.
-  * by rewrite /eq_map_net /= map_app.
+    by rewrite tot_map_name_inv_inverse.
+  * rewrite /= /tot_map_net /=.
+    rewrite -tot_map_update_eq.
+    by rewrite tot_map_packet_eq.
+- apply (@SF_drop _ _ _ _ _ _ (tot_map_packet p) (map tot_map_packet xs) (map tot_map_packet ys)).
+  * by rewrite /tot_map_net /= H4 map_app.
+  * by rewrite /tot_map_net /= map_app.
+- apply (@SF_dup _ _ _ _ _ _ (tot_map_packet p) (map tot_map_packet xs) (map tot_map_packet ys)).
+  * by rewrite /tot_map_net /= H4 map_app.
+  * by rewrite /tot_map_net /= map_app.
 - exact: SF_fail.
-- apply: (SF_reboot (eq_map_name h)).
+- apply: (SF_reboot (tot_map_name h)).
   * exact: in_failed_in.
-  * by rewrite remove_eq_map_eq.
-  * rewrite /eq_map_net /=.
-    by rewrite eq_map_reboot_eq.
+  * by rewrite remove_tot_map_eq.
+  * rewrite /tot_map_net /=.
+    by rewrite tot_map_reboot_eq.
 Qed.
 
-Theorem step_f_eq_mapped_invariant_lift :
+Theorem step_f_tot_mapped_invariant_lift :
   forall P : _ -> Prop,
     (forall net net' failed failed' out,
        @step_f _ _ fail_snd (failed, net) (failed', net') out ->
@@ -610,14 +622,14 @@ Theorem step_f_eq_mapped_invariant_lift :
        P net') ->
     (forall net net' failed failed' out,
        @step_f _ _ fail_fst (failed, net) (failed', net') out ->
-       P (eq_map_net net) ->
-       P (eq_map_net net')).
-Proof. by move => P; eauto using step_f_eq_mapped_simulation_1. Qed.
+       P (tot_map_net net) ->
+       P (tot_map_net net')).
+Proof. by move => P; eauto using step_f_tot_mapped_simulation_1. Qed.
 
-Corollary step_f_mapped_simulation_star_1 :
+Corollary step_f_tot_mapped_simulation_star_1 :
   forall net failed tr,
     @step_f_star _ _ fail_fst step_f_init (failed, net) tr ->
-    @step_f_star _ _ fail_snd step_f_init (map eq_map_name failed, eq_map_net net) (map eq_map_trace_occ tr).
+    @step_f_star _ _ fail_snd step_f_init (map tot_map_name failed, tot_map_net net) (map tot_map_trace_occ tr).
 Proof.
 move => net failed tr H_step.
 remember step_f_init as y in *.
@@ -628,7 +640,7 @@ rewrite {2}H_eq_n {H_eq_n}.
 move: Heqy.
 induction H_step using refl_trans_1n_trace_n1_ind => H_init /=.
   rewrite H_init.
-  rewrite /step_f_init /= /step_m_init /eq_map_net /=.
+  rewrite /step_f_init /= /step_m_init /tot_map_net /=.
   rewrite init_handlers_fun_eq.
   exact: RT1nTBase.
 concludes.
@@ -637,33 +649,18 @@ case: x' H IHH_step1 H_step1 => failed' net'.
 case: x'' H_step2 => failed'' net''.
 rewrite /=.
 move => H_step2 H IHH_step1 H_step1.
-apply step_f_eq_mapped_simulation_1 in H.
+apply step_f_tot_mapped_simulation_1 in H.
 rewrite map_app.
 have H_trans := refl_trans_1n_trace_trans IHH_step1.
 apply: H_trans.
-rewrite (app_nil_end (map eq_map_trace_occ _)).
-apply (@RT1nTStep _ _ _ _ (map eq_map_name failed'', eq_map_net net'')) => //.
+rewrite (app_nil_end (map tot_map_trace_occ _)).
+apply (@RT1nTStep _ _ _ _ (map tot_map_name failed'', tot_map_net net'')) => //.
 exact: RT1nTBase.
 Qed.
 
-(*
-Theorem step_f_eq_mapped_simulation_2 :
-  forall net net' failed failed' out mnet mfailed,
-      @step_f _ _ fail_snd (failed, net) (failed', net') out ->
-      eq_map_net mnet = net ->
-      map eq_map_name mfailed = failed ->
-      exists mnet', exists mfailed', exists mout,
-        @step_f _ _ fail_fst (mfailed, mnet) (mfailed', mnet') mout /\        
-        map eq_map_name mfailed' = failed' /\
-        eq_map_net mnet' = net' /\
-        map eq_map_trace_occ mout = out.
-Proof.
-Admitted.
-*)
-
 Lemma map_eq_name_eq_eq :
   forall l l',
-    map eq_map_name l = map eq_map_name l' -> l = l'.
+    map tot_map_name l = map tot_map_name l' -> l = l'.
 Proof.
 elim.
 case => //=.
@@ -671,25 +668,25 @@ move => n l IH.
 case => //=.
 move => n' l' H_eq.
 inversion H_eq.
-apply eq_map_name_injective in H0.
+apply tot_map_name_injective in H0.
 by rewrite H0 (IH l').
 Qed.
 
-Theorem step_f_eq_mapped_simulation_2 :
+Theorem step_f_tot_mapped_simulation_2 :
   forall net net' failed failed' out mnet mfailed mfailed' mout,
       @step_f _ _ fail_snd (failed, net) (failed', net') out ->
-      eq_map_net mnet = net ->
-      map eq_map_name mfailed = failed ->
-      map eq_map_name mfailed' = failed' ->
-      map eq_map_trace_occ mout = out ->
+      tot_map_net mnet = net ->
+      map tot_map_name mfailed = failed ->
+      map tot_map_name mfailed' = failed' ->
+      map tot_map_trace_occ mout = out ->
       exists mnet',
         @step_f _ _ fail_fst (mfailed, mnet) (mfailed', mnet') mout /\
-        eq_map_net mnet' = net'.
+        tot_map_net mnet' = net'.
 Proof.
 move => net net' failed failed' out mnet mfailed mfailed' mout H_step H_eq_net H_eq_f H_eq_f' H_eq_out.
 invcs H_step.
 - case: p H4 H5 H3 H6 => /= src dst m H4 H5 H3 H6.
-  rewrite /eq_map_net /=.
+  rewrite /tot_map_net /=.
   case: mnet H3 H6 => /= pks sts H_eq H_hnd.
   have [pks1 [pks2 [H_eq_pks [H_eq_pks1 H_eq_pks2]]]] := map_eq_inv _ _ _ _ H_eq.
   case: pks2 H_eq_pks H_eq_pks2 => //= p pks2 H_eq_pks H_eq_pks2.
@@ -700,16 +697,16 @@ invcs H_step.
   rewrite -H_eq_pks1.
   exists {| nwPackets := send_packets (pDst p) l' ++ pks1 ++ pks2 ; nwState := update sts (pDst p) d' |}.
   split.
-  * have [n' [lo [H_eq_mout [H_eq_n H_eq_lo]]]] := eq_map_trace_occ_inv _ (eq_sym H5).
+  * have [n' [lo [H_eq_mout [H_eq_n H_eq_lo]]]] := tot_map_trace_occ_inv _ (eq_sym H5).
     rewrite H_eq_mout.
     have H_eq_dst: n' = pDst p.
-      rewrite -(eq_map_name_inv_inverse n').
+      rewrite -(tot_map_name_inv_inverse n').
       rewrite H_eq_n.
       case: p H_eq_pks H_eq_pks2 H0 H_hnd' => src' dst' m' H_eq_pks H_eq_pks2 H0 H_hnd'.
       rewrite /=.
       rewrite /= in H0.
       inversion H0.
-      by rewrite eq_map_name_inv_inverse.
+      by rewrite tot_map_name_inv_inverse.
     rewrite H_eq_dst.
     apply map_eq_name_eq_eq in H1.
     rewrite H1.    
@@ -720,21 +717,21 @@ invcs H_step.
       by apply in_failed_in in H_in.
     suff H_suff: lo = out' by rewrite H_suff.
     have H_eq_hnd := eq_net_handlers_eq (pDst p) (pSrc p) (pBody p) (sts (pDst p)).
-    rewrite /eq_mapped_net_handlers /= in H_eq_hnd.
+    rewrite /tot_mapped_net_handlers /= in H_eq_hnd.
     repeat break_let.
     inversion H_hnd'.
     rewrite H3 H6 H7 in H_eq_hnd.
     rewrite -{1}H_eq_dst H_eq_n in H_eq_hnd.
     rewrite -H_eq_dst in H_eq_hnd.
-    rewrite -(eq_map_name_inv_inverse n') H_eq_n in H_eq_hnd.
+    rewrite -(tot_map_name_inv_inverse n') H_eq_n in H_eq_hnd.
     move {Heqp1 Heqp0 H_hnd'}.
-    have H_eq_src: eq_map_name (pSrc p) = src.
+    have H_eq_src: tot_map_name (pSrc p) = src.
       case: p H_eq_pks H_eq_pks2 H0 H_eq_dst H_eq_hnd => src' dst' m' H_eq_pks H_eq_pks2 H0 H_eq_dst H_eq_hnd.
       rewrite /=.
       rewrite /= in H0.
       by inversion H0.
     rewrite H_eq_src /= {H_eq_src} in H_eq_hnd.
-    have H_eq_body: eq_map_msg (pBody p) = m.
+    have H_eq_body: tot_map_msg (pBody p) = m.
       case: p H_eq_pks H_eq_pks2 H0 H_eq_dst H_eq_hnd => src' dst' m' H_eq_pks H_eq_pks2 H0 H_eq_dst H_eq_hnd.
       rewrite /=.
       rewrite /= in H0.
@@ -745,33 +742,33 @@ invcs H_step.
     symmetry.
     move: H8.
     apply map_eq_inv_eq.
-    exact: eq_map_output_injective.
+    exact: tot_map_output_injective.
   * rewrite /=.
     rewrite /update /=.
-    have H_eq_dst: eq_map_name (pDst p) = dst.
+    have H_eq_dst: tot_map_name (pDst p) = dst.
       case: p H_eq_pks H_eq_pks2 H0 H_hnd' => src' dst' m' H_eq_pks H_eq_pks2 H0 H_hnd'.
       by inversion H0.
-    have H_eq_src: eq_map_name (pSrc p) = src.
+    have H_eq_src: tot_map_name (pSrc p) = src.
       case: p H_eq_pks H_eq_pks2 H0 H_hnd' H_eq_dst => src' dst' m' H_eq_pks H_eq_pks2 H0 H_hnd' H_eq_dst.
       by inversion H0.
-    have H_eq_body: eq_map_msg (pBody p) = m.
+    have H_eq_body: tot_map_msg (pBody p) = m.
       case: p H_eq_pks H_eq_pks2 H0 H_eq_dst H_eq_src H_hnd' => src' dst' m' H_eq_pks H_eq_pks2 H0 H_eq_dst H_eq_src H_hnd'.
       by inversion H0.
     rewrite 2!map_app.
     have H_eq_hnd := eq_net_handlers_eq (pDst p) (pSrc p) (pBody p) (sts (pDst p)).
-    rewrite /eq_mapped_net_handlers /= in H_eq_hnd.
+    rewrite /tot_mapped_net_handlers /= in H_eq_hnd.
     repeat break_let.
     inversion H_hnd'.
     rewrite H_eq_dst H_eq_src H_eq_body in H_eq_hnd.
-    rewrite -{2}H_eq_dst eq_map_name_inv_inverse in H_hnd.
+    rewrite -{2}H_eq_dst tot_map_name_inv_inverse in H_hnd.
     rewrite H_hnd in H_eq_hnd.
     inversion H_eq_hnd.
     rewrite H3 in H8.
     rewrite H6 in H9.
     rewrite H7 in H10.
     rewrite H6 H7.
-    set nwP1 := map eq_map_packet _.
-    set nwP2 := map (fun _ => _) (eq_map_name_msgs _).
+    set nwP1 := map tot_map_packet _.
+    set nwP2 := map (fun _ => _) (tot_map_name_msgs _).
     set nwS1 := fun _ => _.
     set nwS2 := fun _ => _.
     have H_eq_nw: nwP1 = nwP2.
@@ -787,20 +784,20 @@ invcs H_step.
       rewrite -H_eq_dst.
       case (name_eq_dec _ _) => H_dec.
         rewrite -H_dec.
-        rewrite eq_map_name_inverse_inv.
+        rewrite tot_map_name_inverse_inv.
         by case (name_eq_dec _ _).
       case (name_eq_dec _ _) => H_dec' //.
       rewrite H_dec' in H_dec.
-      by rewrite eq_map_name_inv_inverse in H_dec.
+      by rewrite tot_map_name_inv_inverse in H_dec.
     by rewrite H_eq_sw.
-- rewrite /eq_map_net /=.
+- rewrite /tot_map_net /=.
   case: mnet H5 => /= pks sts H_hnd.
-  have [h' [inp' [out' [H_eq_mout [H_eq_n [H_eq_out H_eq_inp]]]]]] := eq_map_trace_occ_in_inv _ (eq_sym H4).
+  have [h' [inp' [out' [H_eq_mout [H_eq_n [H_eq_out H_eq_inp]]]]]] := tot_map_trace_occ_in_inv _ (eq_sym H4).
   have H_q := eq_input_handlers_eq h' inp' (sts h').
-  rewrite /eq_mapped_input_handlers in H_q.
+  rewrite /tot_mapped_input_handlers in H_q.
   repeat break_let.
   rewrite H_eq_n H_eq_inp in H_q.
-  rewrite -{2}H_eq_n eq_map_name_inv_inverse in H_hnd.
+  rewrite -{2}H_eq_n tot_map_name_inv_inverse in H_hnd.
   rewrite H_hnd in H_q.
   inversion H_q.
   rewrite -H_eq_out in H0.
@@ -819,9 +816,9 @@ invcs H_step.
     suff H_suff: l1 = out' by rewrite H_suff.
     move: H0.
     apply map_eq_inv_eq.
-    exact: eq_map_output_injective.
+    exact: tot_map_output_injective.
   * rewrite /= map_app.
-    set nwP1 := map eq_map_packet _.
+    set nwP1 := map tot_map_packet _.
     set nwP2 := map (fun _ => _) l.
     set nwS1 := fun _ => _.
     set nwS2 := update _ _ _.
@@ -838,9 +835,9 @@ invcs H_step.
       rewrite -H_eq_n -H2.
       case (name_eq_dec _ _) => H_dec.
         case (name_eq_dec _ _) => H_dec' //.
-        by rewrite -H_dec eq_map_name_inverse_inv in H_dec'.
+        by rewrite -H_dec tot_map_name_inverse_inv in H_dec'.
       case (name_eq_dec _ _) => H_dec' //.
-      by rewrite H_dec' eq_map_name_inv_inverse in H_dec.
+      by rewrite H_dec' tot_map_name_inv_inverse in H_dec.
     by rewrite H_eq_nwp H_eq_nws.
 - case: mout H2 => // H_eq_mout {H_eq_mout}.
   apply map_eq_name_eq_eq in H1.
@@ -851,7 +848,7 @@ invcs H_step.
   rewrite -H_eq_pks1.
   exists {| nwPackets := pks1 ++ pks2 ; nwState := nwState mnet |}.
   split; first exact: (@SF_drop _ _ _ _ _ _ p' pks1 pks2).
-  by rewrite /eq_map_net /= map_app.
+  by rewrite /tot_map_net /= map_app.
 - case: mout H2 => // H_eq_mout {H_eq_mout}.
   apply map_eq_name_eq_eq in H1.
   rewrite -H1.
@@ -861,7 +858,7 @@ invcs H_step.
   rewrite -H_eq_pks1.
   exists {| nwPackets := p' :: pks1 ++ p' :: pks2 ; nwState := nwState mnet |}.
   split; first exact: (@SF_dup _ _ _ _ _ _ p' pks1 pks2).
-  by rewrite /eq_map_net /= map_app.
+  by rewrite /tot_map_net /= map_app.
 - case: mout H2 => // H_eq_mout {H_eq_mout}.
   case: mfailed' H => //= h' mfailed' H_eq.
   inversion H_eq.
@@ -889,17 +886,17 @@ invcs H_step.
     + inversion H_eq_mns2.
       rewrite -H0 in H5.
       move {H3 ns1 ns2 H_eq mns1 H_eq_mns1 h mns2 H_eq_mns H_eq_mns2 H0 H1}.
-      have H_eq: remove name_eq_dec (eq_map_name h') (map eq_map_name mfailed) = map eq_map_name (remove name_eq_dec h' mfailed).
+      have H_eq: remove name_eq_dec (tot_map_name h') (map tot_map_name mfailed) = map tot_map_name (remove name_eq_dec h' mfailed).
         move {H5 mfailed'}.
         elim: mfailed => //=.
         move => n l IH.
         case (name_eq_dec _ _) => H_dec; case (name_eq_dec _ _) => H_dec' => //.
-        + by apply eq_map_name_injective in H_dec.
+        + by apply tot_map_name_injective in H_dec.
         + by rewrite H_dec' in H_dec.
         + by rewrite /= IH.               
       rewrite H_eq in H5.
       by apply map_eq_name_eq_eq in H5.
-  * rewrite /eq_map_net /=.
+  * rewrite /tot_map_net /=.
     inversion H_eq_mns2.
     set nwS1 := fun _ => _.
     set nwS2 := fun _ => _.
@@ -908,13 +905,13 @@ invcs H_step.
       apply functional_extensionality => n.
       case (name_eq_dec _ _) => H_dec; case (name_eq_dec _ _) => H_dec' => //.
       + rewrite -H_dec in H_dec'.
-        by rewrite eq_map_name_inverse_inv in H_dec'.
+        by rewrite tot_map_name_inverse_inv in H_dec'.
       + rewrite H_dec' in H_dec.
-        by rewrite eq_map_name_inv_inverse in H_dec.
+        by rewrite tot_map_name_inv_inverse in H_dec.
     by rewrite H_eq_sw.
 Qed.
 
-End SimulOneToOne.
+End SimulTot.
 
 Section GhostVars.
 
@@ -986,43 +983,33 @@ Defined.
 
 Arguments deghost_packet /_.
 
-Instance refined_base_params_eq_map : BaseParamsEqMap refined_base_params base_params :=
+Instance refined_base_params_tot_map : BaseParamsTotMap refined_base_params base_params :=
   {
-    eq_map_data := snd ;
-    eq_map_input := id ;
-    eq_map_output := id
+    tot_map_data := snd ;
+    tot_map_input := id ;
+    tot_map_output := id
   }.
 
-Instance refined_multi_params_eq_map : MultiParamsEqMap refined_base_params_eq_map refined_multi_params multi_params :=
+Instance refined_multi_params_tot_map : MultiParamsTotMap refined_base_params_tot_map refined_multi_params multi_params :=
   {
-    eq_map_msg := id ;
-    eq_map_name := id ;
-    eq_map_name_inv := id ;
-    eq_map_name_inv_inverse := fun n => eq_refl ;
-    eq_map_name_inverse_inv := fun n => eq_refl
+    tot_map_msg := id ;
+    tot_map_name := id ;
+    tot_map_name_inv := id
   }.
 
-Lemma hyp_eq_mapped_init_handlers_eq : forall n,
-  eq_mapped_init_handlers n = init_handlers (eq_map_name n).
+Lemma ghost_tot_map_name_inv_inverse : forall n, tot_map_name_inv (tot_map_name n) = n.
 Proof. by []. Qed.
 
-Lemma map_fst_snd_id : 
-  forall A B l, map (fun t : A * B => (fst t, snd t)) l = l.
-Proof.
-move => A B.
-elim => //.
-move => a l IH.
-rewrite /= IH.
-by case: a.
-Qed.
+Lemma ghost_tot_map_name_inverse_inv : forall n, tot_map_name (tot_map_name_inv n) = n.
+Proof. by []. Qed.
 
-Lemma hyp_eq_net_handlers_eq : 
+Lemma ghost_eq_net_handlers_eq : 
   forall me src m st,
-    eq_mapped_net_handlers me src m st = 
-    net_handlers (eq_map_name me) (eq_map_name src) (eq_map_msg m) (eq_map_data st).
+    tot_mapped_net_handlers me src m st = 
+    net_handlers (tot_map_name me) (tot_map_name src) (tot_map_msg m) (tot_map_data st).
 Proof.
 move => me src m st.
-rewrite /eq_mapped_net_handlers /= /refined_net_handlers /= /eq_map_name_msgs /= /id /=.
+rewrite /tot_mapped_net_handlers /= /refined_net_handlers /= /tot_map_name_msgs /= /id /=.
 repeat break_let.
 move {p0 Heqp1 p Heqp2}.
 inversion Heqp; subst.
@@ -1032,23 +1019,23 @@ rewrite map_id.
 by rewrite map_fst_snd_id.
 Qed.
 
-Lemma hyp_eq_input_handlers_eq : forall me inp st,
-  eq_mapped_input_handlers me inp st = input_handlers (eq_map_name me) (eq_map_input inp) (eq_map_data st).
+Lemma ghost_eq_input_handlers_eq : forall me inp st,
+  tot_mapped_input_handlers me inp st = input_handlers (tot_map_name me) (tot_map_input inp) (tot_map_data st).
 Proof.
 move => me inp st.
-rewrite /eq_mapped_input_handlers /=.
+rewrite /tot_mapped_input_handlers /=.
 repeat break_let.
 rewrite map_id.
 rewrite /refined_input_handlers in Heqp.
 repeat break_let.
 rewrite /id /= Heqp1.
 inversion Heqp; subst.
-rewrite /= /eq_map_name_msgs /= /id /=.
+rewrite /= /tot_map_name_msgs /= /id /=.
 by rewrite map_fst_snd_id.
 Qed.
 
-Lemma hyp_eq_mapped_reboot_eq : forall d,
-  eq_map_data (reboot d) = reboot (eq_map_data d).
+Lemma ghost_tot_mapped_reboot_eq : forall d,
+  tot_map_data (reboot d) = reboot (tot_map_data d).
 Proof. by []. Qed.
 
 Lemma map_id_tr :
@@ -1073,12 +1060,12 @@ Theorem ghost_simulation_1 :
     @step_f _ _ refined_failure_params (failed, net) (failed', net') out ->
     @step_f _ _ failure_params (failed, deghost net) (failed', deghost net') out.
 Proof.
-have H_sim := step_f_eq_mapped_simulation_1 hyp_eq_net_handlers_eq hyp_eq_input_handlers_eq hyp_eq_mapped_reboot_eq.
+have H_sim := step_f_tot_mapped_simulation_1 ghost_tot_map_name_inv_inverse ghost_tot_map_name_inverse_inv ghost_eq_net_handlers_eq ghost_eq_input_handlers_eq ghost_tot_mapped_reboot_eq.
 move => net net' failed failed' out H_step.
 apply H_sim in H_step.
-rewrite /eq_map_name /eq_map_net /= 2!map_id /id /= in H_step.
-rewrite /eq_map_trace_occ /= /id /= in H_step.
-rewrite /eq_map_packet /= /id /= in H_step.
+rewrite /tot_map_name /tot_map_net /= 2!map_id /id /= in H_step.
+rewrite /tot_map_trace_occ /= /id /= in H_step.
+rewrite /tot_map_packet /= /id /= in H_step.
 rewrite /deghost /=.
 rewrite -/id map_id_tr in H_step.
 move: H_step.
@@ -1096,8 +1083,22 @@ have H_eq: fs2 = fs2' by rewrite /fs2 /fs2' {fs2 fs2'}; apply functional_extensi
 by rewrite H_eq {H_eq fs2}.
 Qed.
 
-Lemma hyp_eq_map_output_injective : 
-  forall o o', eq_map_output o = eq_map_output o' -> o = o'.
+Theorem ghost_invariant_lift :
+  forall P : _ -> Prop,
+    (forall net net' failed failed' out,
+       @step_f _ _ failure_params (failed, net) (failed', net') out ->
+       P net ->
+       P net') ->
+    (forall net net' failed failed' out,
+       step_f (failed, net) (failed', net') out ->
+       P (deghost net) ->
+       P (deghost net')).
+Proof.
+  intros. eauto using ghost_simulation_1.
+Qed.
+
+Lemma ghost_tot_map_output_injective : 
+  forall o o', tot_map_output o = tot_map_output o' -> o = o'.
 Proof. by []. Qed.
 
 Theorem ghost_simulation_2 :
@@ -1108,14 +1109,14 @@ Theorem ghost_simulation_2 :
       step_f (failed, gnet) (failed', gnet') out /\
       deghost gnet' = net'.
 Proof.
-have H_sim := step_f_eq_mapped_simulation_2 hyp_eq_net_handlers_eq hyp_eq_input_handlers_eq hyp_eq_map_output_injective hyp_eq_mapped_reboot_eq.
+have H_sim := step_f_tot_mapped_simulation_2 ghost_tot_map_name_inv_inverse ghost_tot_map_name_inverse_inv ghost_eq_net_handlers_eq ghost_eq_input_handlers_eq ghost_tot_map_output_injective ghost_tot_mapped_reboot_eq.
 move => net net' failed failed' out gnet H_step H_eq.
 apply (H_sim _ _ _ _ _ gnet failed failed' out) in H_step.
 - move: H_step => [gnet' [H_step H_eq_net]].
   exists gnet'.
   split => //.
   rewrite -H_eq_net {H_step H_eq_net}.
-  rewrite /deghost /eq_map_net /= /id /= /eq_map_packet /= /id /=.
+  rewrite /deghost /tot_map_net /= /id /= /tot_map_packet /= /id /=.
   set nwPf1 := fun p : packet => _.
   set nwPf2 := fun p : packet => _.
   have H_eq_p: nwPf1 = nwPf2 by rewrite /nwPf1 /nwPf2 {nwPf1 nwPf2}; apply functional_extensionality; case.
@@ -1123,7 +1124,7 @@ apply (H_sim _ _ _ _ _ gnet failed failed' out) in H_step.
   set nwS2 := fun _ => _.
   have H_eq_s: nwS1 = nwS2 by rewrite /nwS1 /nwS2 {nwS1 nwS2}; apply functional_extensionality => n; case: gnet'.
   by rewrite H_eq_p H_eq_s.
-- rewrite /eq_map_net /= /id /= /eq_map_packet /= /id /=.
+- rewrite /tot_map_net /= /id /= /tot_map_packet /= /id /=.
   move: H_eq.
   rewrite /deghost /=.
   set nwPf1 := fun p : packet => _.
@@ -1133,8 +1134,8 @@ apply (H_sim _ _ _ _ _ gnet failed failed' out) in H_step.
   set nwS2 := fun _ => _.
   have H_eq_s: nwS1 = nwS2 by rewrite /nwS1 /nwS2 {nwS1 nwS2}; apply functional_extensionality => n; case: gnet.
   by rewrite H_eq_p H_eq_s.
-- by rewrite /eq_map_name /= map_id.
-- by rewrite /eq_map_name /= map_id.
+- by rewrite /tot_map_name /= map_id.
+- by rewrite /tot_map_name /= map_id.
 - move {H_step}.
   elim: out => //.
   case => n t out IH.
@@ -1144,6 +1145,54 @@ apply (H_sim _ _ _ _ _ gnet failed failed' out) in H_step.
     by rewrite IH.
   move => out'.
   by rewrite {1}/id map_id /= IH.
+Qed.
+
+Definition ghost_packet p :=
+  @mkPacket _ refined_multi_params
+            (@pSrc _ multi_params p)
+            (pDst p)
+            (pBody p).
+
+Arguments ghost_packet /_.
+
+Definition reghost (net : @network _ multi_params) : @network _ refined_multi_params.
+  refine (@mkNetwork _ refined_multi_params
+                     (map ghost_packet
+                        (nwPackets net))
+                     _
+         ).
+  intros.
+  destruct net.
+  concludes.
+  exact (ghost_init, nwState).
+Defined.
+
+Lemma reghost_deghost_partial_inverses :
+  forall net,
+    deghost (reghost net) = net.
+Proof.
+  destruct net. unfold deghost, reghost. simpl in *. f_equal.
+  rewrite map_map. map_id.
+Qed.
+
+Theorem ghost_invariant_lower :
+  forall P : _ -> Prop,
+    (forall net net' failed failed' out,
+       step_f (failed, net) (failed', net') out ->
+       P (deghost net) ->
+       P (deghost net')) ->
+    (forall net net' failed failed' out,
+       @step_f _ _ failure_params (failed, net) (failed', net') out ->
+       P net ->
+       P net').
+Proof.
+  intros.
+  apply ghost_simulation_2 with (gnet := reghost net) in H0.
+  - break_exists. intuition. subst.
+    eapply H; eauto.
+    rewrite reghost_deghost_partial_inverses.
+    auto.
+  - eauto using reghost_deghost_partial_inverses.
 Qed.
 
 End GhostVars.
@@ -1221,33 +1270,33 @@ Definition add_ghost_msg (me : name) (st : data) (ps : list (name * msg)) :
 
   Arguments mgv_deghost_packet /_.
 
-Instance mgv_refined_base_params_eq_map : BaseParamsEqMap mgv_refined_base_params base_params :=
+Instance mgv_refined_base_params_tot_map : BaseParamsTotMap mgv_refined_base_params base_params :=
   {
-    eq_map_data := id ;
-    eq_map_input := id ;
-    eq_map_output := id
+    tot_map_data := id ;
+    tot_map_input := id ;
+    tot_map_output := id
   }.
 
-Instance mgv_refined_multi_params_eq_map : MultiParamsEqMap mgv_refined_base_params_eq_map mgv_refined_multi_params multi_params :=
+Instance mgv_refined_multi_params_tot_map : MultiParamsTotMap mgv_refined_base_params_tot_map mgv_refined_multi_params multi_params :=
   {
-    eq_map_msg := snd ;
-    eq_map_name := id ;
-    eq_map_name_inv := id ;
-    eq_map_name_inv_inverse := fun n => eq_refl ;
-    eq_map_name_inverse_inv := fun n => eq_refl
+    tot_map_msg := snd ;
+    tot_map_name := id ;
+    tot_map_name_inv := id
   }.
 
-Lemma mgv_hyp_eq_mapped_init_handlers_eq : forall n,
-  eq_mapped_init_handlers n = init_handlers (eq_map_name n).
+Lemma mgv_tot_map_name_inv_inverse : forall n, tot_map_name_inv (tot_map_name n) = n.
 Proof. by []. Qed.
 
-Lemma mgv_hyp_eq_net_handlers_eq : 
+Lemma mgv_tot_map_name_inverse_inv : forall n, tot_map_name (tot_map_name_inv n) = n.
+Proof. by []. Qed.
+
+Lemma mgv_eq_net_handlers_eq : 
   forall me src m st,
-    eq_mapped_net_handlers me src m st = 
-    net_handlers (eq_map_name me) (eq_map_name src) (eq_map_msg m) (eq_map_data st).
+    tot_mapped_net_handlers me src m st = 
+    net_handlers (tot_map_name me) (tot_map_name src) (tot_map_msg m) (tot_map_data st).
 Proof.
 move => me src m st.
-rewrite /eq_mapped_net_handlers /= /mgv_refined_net_handlers /= /eq_map_name_msgs /= /id /=.
+rewrite /tot_mapped_net_handlers /= /mgv_refined_net_handlers /= /tot_map_name_msgs /= /id /=.
 repeat break_let.
 rewrite -/id map_id.
 inversion Heqp; subst.
@@ -1261,17 +1310,17 @@ move => IH'.
 by rewrite IH'.
 Qed.
 
-Lemma mgv_hyp_eq_input_handlers_eq : forall me inp st,
-  eq_mapped_input_handlers me inp st = input_handlers (eq_map_name me) (eq_map_input inp) (eq_map_data st).
+Lemma mgv_eq_input_handlers_eq : forall me inp st,
+  tot_mapped_input_handlers me inp st = input_handlers (tot_map_name me) (tot_map_input inp) (tot_map_data st).
 Proof.
 move => me inp st.
-rewrite /eq_mapped_input_handlers /=.
+rewrite /tot_mapped_input_handlers /=.
 repeat break_let.
 rewrite map_id /id /=.
 rewrite /mgv_refined_input_handlers in Heqp.
 repeat break_let.
 inversion Heqp; subst.
-rewrite /= /eq_map_name_msgs /= /id /=.
+rewrite /= /tot_map_name_msgs /= /id /=.
 move {Heqp1 Heqp}.
 elim: l1 => //.
 case => n m l.
@@ -1282,8 +1331,8 @@ move => IH'.
 by rewrite IH'.
 Qed.
 
-Lemma mgv_hyp_eq_mapped_reboot_eq : forall d,
-  eq_map_data (reboot d) = reboot (eq_map_data d).
+Lemma mgv_tot_mapped_reboot_eq : forall d,
+  tot_map_data (reboot d) = reboot (tot_map_data d).
 Proof. by []. Qed.
 
 Lemma mgv_map_id_tr :
@@ -1308,12 +1357,12 @@ Theorem mgv_ghost_simulation_1 :
     @step_f _ _ mgv_refined_failure_params (failed, net) (failed', net') out ->
     @step_f _ _ failure_params (failed, mgv_deghost net) (failed', mgv_deghost net') out.
 Proof.
-have H_sim := step_f_eq_mapped_simulation_1 mgv_hyp_eq_net_handlers_eq mgv_hyp_eq_input_handlers_eq mgv_hyp_eq_mapped_reboot_eq.
+have H_sim := step_f_tot_mapped_simulation_1 mgv_tot_map_name_inv_inverse mgv_tot_map_name_inverse_inv mgv_eq_net_handlers_eq mgv_eq_input_handlers_eq mgv_tot_mapped_reboot_eq.
 move => net net' failed failed' out H_step.
 apply H_sim in H_step.
-rewrite /eq_map_name /eq_map_net /= 2!map_id /id /= in H_step.
-rewrite /eq_map_trace_occ /= /id /= in H_step.
-rewrite /eq_map_packet /= /id /= in H_step.
+rewrite /tot_map_name /tot_map_net /= 2!map_id /id /= in H_step.
+rewrite /tot_map_trace_occ /= /id /= in H_step.
+rewrite /tot_map_packet /= /id /= in H_step.
 rewrite /mgv_deghost /=.
 rewrite -/id mgv_map_id_tr in H_step.
 move: H_step.
@@ -1331,8 +1380,8 @@ have H_eq: fs2 = fs2' by rewrite /fs2 /fs2' {fs2 fs2'}; apply functional_extensi
 by rewrite H_eq {H_eq fs2}.
 Qed.
 
-Lemma mgv_hyp_eq_map_output_injective : 
-  forall o o', eq_map_output o = eq_map_output o' -> o = o'.
+Lemma mgv_tot_map_output_injective : 
+  forall o o', tot_map_output o = tot_map_output o' -> o = o'.
 Proof. by []. Qed.
 
 Theorem mgv_ghost_simulation_2 :
@@ -1343,14 +1392,14 @@ Theorem mgv_ghost_simulation_2 :
       step_f (failed, gnet) (failed', gnet') out /\
       mgv_deghost gnet' = net'.
 Proof.
-have H_sim := step_f_eq_mapped_simulation_2 mgv_hyp_eq_net_handlers_eq mgv_hyp_eq_input_handlers_eq mgv_hyp_eq_map_output_injective mgv_hyp_eq_mapped_reboot_eq.
+have H_sim := step_f_tot_mapped_simulation_2 mgv_tot_map_name_inv_inverse mgv_tot_map_name_inverse_inv mgv_eq_net_handlers_eq mgv_eq_input_handlers_eq mgv_tot_map_output_injective mgv_tot_mapped_reboot_eq.
 move => net net' failed failed' out gnet H_step H_eq.
 apply (H_sim _ _ _ _ _ gnet failed failed' out) in H_step.
 - move: H_step => [gnet' [H_step H_eq_net]].
   exists gnet'.
   split => //.
   rewrite -H_eq_net {H_step H_eq_net}.
-  rewrite /mgv_deghost /eq_map_net /= /id /= /eq_map_packet /= /id /=.
+  rewrite /mgv_deghost /tot_map_net /= /id /= /tot_map_packet /= /id /=.
   set nwPf1 := fun p : packet => _.
   set nwPf2 := fun p : packet => _.
   have H_eq_p: nwPf1 = nwPf2 by rewrite /nwPf1 /nwPf2 {nwPf1 nwPf2}; apply functional_extensionality; case.
@@ -1359,7 +1408,7 @@ apply (H_sim _ _ _ _ _ gnet failed failed' out) in H_step.
   have H_eq_s: nwS1 = nwS2 by rewrite /nwS1 /nwS2 {nwS1 nwS2}; apply functional_extensionality => n; case: gnet'.
   by rewrite H_eq_p H_eq_s.
 - rewrite -H_eq {H_step H_eq}.
-  rewrite /mgv_deghost /eq_map_net /= /id /= /eq_map_packet /= /id /=.
+  rewrite /mgv_deghost /tot_map_net /= /id /= /tot_map_packet /= /id /=.
   set nwPf1 := fun p : packet => _.
   set nwPf2 := fun p : packet => _.
   have H_eq_p: nwPf1 = nwPf2 by rewrite /nwPf1 /nwPf2 {nwPf1 nwPf2}; apply functional_extensionality; case.
@@ -1367,8 +1416,8 @@ apply (H_sim _ _ _ _ _ gnet failed failed' out) in H_step.
   set nwS2 := fun _ => _.
   have H_eq_s: nwS1 = nwS2 by rewrite /nwS1 /nwS2 {nwS1 nwS2}; apply functional_extensionality => n; case: gnet.
   by rewrite H_eq_p H_eq_s.
-- by rewrite /eq_map_name /= map_id.
-- by rewrite /eq_map_name /= map_id.
+- by rewrite /tot_map_name /= map_id.
+- by rewrite /tot_map_name /= map_id.
 - move {H_step}.
   elim: out => //.
   case => n t out IH.
@@ -1380,32 +1429,53 @@ apply (H_sim _ _ _ _ _ gnet failed failed' out) in H_step.
   by rewrite {1}/id map_id /= IH.
 Qed.
 
-(*
-Definition ghost_packet p :=
-  @mkPacket _ refined_multi_params
+Definition mgv_ghost_packet p :=
+  @mkPacket _ mgv_refined_multi_params
             (@pSrc _ multi_params p)
             (pDst p)
-            (pBody p).
+            (ghost_msg_default, pBody p).
 
-Arguments ghost_packet /_.
 
-Definition reghost (net : @network _ multi_params) : @network _ refined_multi_params.
-  refine (@mkNetwork _ refined_multi_params
-                     (map ghost_packet
+Definition mgv_reghost (net : @network _ multi_params) : @network _ mgv_refined_multi_params.
+  refine (@mkNetwork _ mgv_refined_multi_params
+                     (map mgv_ghost_packet
                         (nwPackets net))
                      _
          ).
   intros.
   destruct net.
   concludes.
-  exact (ghost_init, nwState).
+  auto.
 Defined.
 
-Lemma reghost_deghost_partial_inverses :
+Arguments mgv_ghost_packet /_.
+
+Lemma mgv_reghost_deghost_partial_inverses :
   forall net,
-    deghost (reghost net) = net.
+    mgv_deghost (mgv_reghost net) = net.
 Proof.
-  destruct net. unfold deghost, reghost. simpl in *. f_equal.
+  destruct net. unfold mgv_deghost, mgv_reghost. simpl in *. f_equal.
   rewrite map_map. map_id.
 Qed.
-*)
+
+Theorem mgv_ghost_invariant_lower :
+  forall P : _ -> Prop,
+    (forall net net' failed failed' out,
+       step_f (failed, net) (failed', net') out ->
+       P (mgv_deghost net) ->
+       P (mgv_deghost net')) ->
+    (forall net net' failed failed' out,
+       @step_f _ _ failure_params (failed, net) (failed', net') out ->
+       P net ->
+       P net').
+Proof.
+  intros.
+  apply mgv_ghost_simulation_2 with (gnet := mgv_reghost net) in H0.
+  - break_exists. intuition. subst.
+    eapply H; eauto.
+    rewrite mgv_reghost_deghost_partial_inverses.
+    auto.
+  - eauto using mgv_reghost_deghost_partial_inverses.
+Qed.
+
+End MsgGhostVars.
